thy/Abstract_Impl.thy
@@ -27,54 +27,19 @@ locale bdd_impl = bdd_impl_pre R for R :: "'s \<Rightarrow> ('ni \<times> ('a ::
   assumes Timpl_rule: "Timpl s = (ni, s') \<Longrightarrow> (ni, Trueif) \<in> R s'"
   assumes Fimpl_rule: "Fimpl s = (ni, s') \<Longrightarrow> (ni, Falseif) \<in> R s'"
   assumes IFimpl_rule: "\<lbrakk>(ni1,n1) \<in> R s;(ni2,n2) \<in> R s; IFimpl v ni1 ni2 s = (ni, s')\<rbrakk>
-                       \<Longrightarrow> (ni, IF v n1 n2) \<in> R s'"
+                       \<Longrightarrow> (ni, IFC v n1 n2) \<in> R s'"
 
   assumes DESTRimpl_rule1: "(ni, Trueif) \<in> R s \<Longrightarrow> DESTRimpl ni s = TD"
   assumes DESTRimpl_rule2: "(ni, Falseif) \<in> R s \<Longrightarrow> DESTRimpl ni s = FD"
   assumes DESTRimpl_rule3: "(ni, IF v n1 n2) \<in> R s \<Longrightarrow> \<exists>ni1 ni2. DESTRimpl ni s = IFD v ni1 ni2 
                                                        \<and> (ni1, n1) \<in> R s \<and> (ni2, n2) \<in> R s"
+                                                       
+  assumes rel_minimal: "(ni,n) \<in> R s \<Longrightarrow> ifex_minimal n" 
 
 begin
 
-
-function restrict_impl where
-  "restrict_impl n var val s = (case DESTRimpl n s of
-                                    (IFD v t e) \<Rightarrow> (let (rt,s) = restrict_impl t var val s;
-                                                        (re,s) = restrict_impl e var val s in
-                                                     if v = var then (if val then (rt,s) else (re, s)) else
-                                                     (IFimpl v rt re s)) |
-                                     i \<Rightarrow> (n,s))"
-by pat_completeness auto
-
-partial_function(option) restrict_impl_opt where
-  "restrict_impl_opt n var val s = (case DESTRimpl n s of
-                                    (IFD v t e) \<Rightarrow> (do {(rt,s) \<leftarrow> restrict_impl_opt t var val s;
-                                                        (re,s) \<leftarrow> restrict_impl_opt e var val s;
-                                                     if v = var then (if val then Some (rt,s) else Some (re, s)) else
-                                                     Some (IFimpl v rt re s)}) |
-                                     _ \<Rightarrow> Some (n,s))"
-
 lemma les_refl[simp,intro!]:"les s s" by (auto simp add: les_def)
 lemma les_trans[trans]:"les s1 s2 \<Longrightarrow> les s2 s3 \<Longrightarrow> les s1 s3" by (auto simp add: les_def)
-
-
-lemma "(ni, n) \<in> R s \<Longrightarrow> \<exists>rni s'. restrict_impl_opt ni var val s = Some (rni, s') \<and> 
-                          (rni, restrict n var val) \<in> R s' \<and> les s s'"
-proof(induction n arbitrary: ni s)
-	case goal3
-	note DESTRimpl_rule3[OF goal3(3)] then obtain ni1 ni2 where dimp: "DESTRimpl ni s = IFD x1 ni1 ni2" and ni1: "(ni1, n1) \<in> R s" and ni2: "(ni2, n2) \<in> R s" by blast
-	note goal3(1)[OF ni1]
-	then obtain rnit s' where rnits: "restrict_impl_opt ni1 var val s = Some (rnit, s')" "(rnit, restrict n1 var val) \<in> R s'" "les s s'" by blast
-	from this(3) ni2 have "(ni2, n2) \<in> R s'" unfolding les_def by simp
-	note goal3(2)[OF this]
-	then obtain rnie s'' where rnies: "restrict_impl_opt ni2 var val s' = Some (rnie, s'')" "(rnie, restrict n2 var val) \<in> R s''"  "les s' s''" by blast
-	from this(3) rnits(2) have 1: "(rnit, restrict n1 var val) \<in> R s''" unfolding les_def by simp
-	obtain r s''' where rs: "IFimpl x1 rnit rnie s'' = (r,s''')" by force
-	have les: "les s s''" "les s s'''" using les_trans rnits(3) rnies(3) IFimpl_mono[OF 1 rnies(2) rs] by blast+
-	show ?case
-		using 1 rnies(2) les IFimpl_rule[OF 1 rnies(2) rs]
-		by(subst restrict_impl_opt.simps, auto simp add: rnits(1) rnies(1) dimp rs)
-qed (force dest: DESTRimpl_rule1 DESTRimpl_rule2 simp add: restrict_impl_opt.simps)+
 
 fun lowest_tops_impl where
 "lowest_tops_impl [] s = None" |
@@ -136,9 +101,7 @@ partial_function(option) ite_impl where
             Some (IFimpl a tb fb s)}) |
         None \<Rightarrow> Some (case DESTRimpl i s of TD \<Rightarrow> (t, s) | FD \<Rightarrow> (e, s)))"
 
-thm ite_impl.raw_induct (* Ask lars about induction over ite_impl *)
-
-lemma "ite_impl ii ti ei s = Some (r, s')
+lemma ite_impl_R: "ite_impl ii ti ei s = Some (r, s')
        \<Longrightarrow> in_R_list [ii, ti, ei] [i, t, e] s
        \<Longrightarrow> les s s' \<and> (r, ifex_ite i t e) \<in> R s'"
 proof(induction i t e arbitrary: s s' ii ti ei r rule: ifex_ite_induct)
@@ -189,11 +152,12 @@ case ("3" i t e a)
   from IFCase(2)
     have 7:
     "ifex_ite i t e =
-     IF a (ifex_ite (restrict_top i a True) (restrict_top t a True) (restrict_top e a True))
+     IFC a (ifex_ite (restrict_top i a True) (restrict_top t a True) (restrict_top e a True))
       (ifex_ite (restrict_top i a False) (restrict_top t a False) (restrict_top e a False))"
     by simp
   from 5 IFCase(3) have "IFimpl a tb eb se = (r, s')" by force
-  from goal11 IFimpl_rule[OF 8 4(1) this] 7 show ?case by presburger
+  from goal11 IFimpl_rule[OF 8 4(1) this] 7 show ?case
+  by(auto split: ifc_split dest: rel_minimal)
 next
 case("1" i t e) note TrueIFCase = "1"
   from in_R_list_lt[OF this(4)] this(1,2,4) DESTRimpl_rule1
